Incorporate continuations into Process

src/Verifier/Verifier.dfy
@@ -6,6 +6,7 @@ module Verifier {
   import RSolvers
   import StaticConsistency
   import AssignmentTargets
+  import BC = BlockContinuations
 
   export
     provides Verify
@@ -37,11 +38,9 @@ module Verifier {
     // Assume precondition (TODO: should also vet precondition)
     context := AssumeAExprs(proc.Post, preIncarnations, context, smtEngine);
 
-    if proc.Body.Some? {
-      var cp;
-      bodyIncarnations, context, cp := ProcessStmt(proc.Body.value, bodyIncarnations, context, smtEngine);
-      expect cp == Normal, cp; // TODO: this holds if all exit in the body go to defined labels
-    }
+    var body := if proc.Body.Some? then [proc.Body.value] else [];
+    Process(body, bodyIncarnations, context, BC.Empty(), smtEngine);
+    // TODO: postcondition checking should be appended to body, not checked separately
 
     // Check postcondition (TODO: should also vet postcondition)
     CheckAExprs(proc.Post, bodyIncarnations, context, smtEngine, "postcondition");
@@ -86,6 +85,10 @@ module Verifier {
       Incarnations(map[], map[])
     }
 
+    function Variables(): set<Variable> {
+      m.Keys
+    }
+
     // `Set` is intended to be used only during custom initializations of an Incarnations.
     function Set(v: Variable, sv: SVar): Incarnations {
       Incarnations(map[v.name := 0] + nextSequenceCount, m[v := sv])
@@ -105,6 +108,11 @@ module Verifier {
       incarnations := Incarnations(nextSequenceCount[v.name := nextSequenceNumber], m[v := x]);
     }
 
+    function DomainRestrict(variables: set<Variable>): Incarnations {
+      var m' := map v <- m.Keys | v in variables :: m[v];
+      Incarnations(nextSequenceCount, m')
+    }
+
     function REval(expr: Expr): RSolvers.RExpr {
       match expr
       case BConst(value) => RExpr.Boolean(value)
@@ -120,19 +128,19 @@ module Verifier {
     }
   }
 
-  datatype ContinuationPoint =
-    | Normal
-    | Abrupt(lbl: Label)
-    | NoExit
-
-  method ProcessStmt(stmt: Stmt, incarnations_in: Incarnations, context_in: RSolvers.RContext, smtEngine: RSolvers.REngine)
-      returns (incarnations: Incarnations, context: RSolvers.RContext, cp: ContinuationPoint)
+  method Process(stmts: seq<Stmt>, incarnations_in: Incarnations, context_in: RSolvers.RContext, B: BC.T, smtEngine: RSolvers.REngine)
     requires smtEngine.Valid()
     modifies smtEngine.Repr
     ensures smtEngine.Valid()
-    decreases stmt
+    decreases BC.StmtSeqMeasure(stmts) + BC.ContinuationsMeasure(B)
   {
-    incarnations, context, cp := incarnations_in, context_in, Normal;
+    if stmts == [] {
+      return;
+    }
+
+    var incarnations, context := incarnations_in, context_in;
+    var stmt, cont := stmts[0], stmts[1..];
+    BC.StmtMeasureSplit(stmts);
     match stmt
     case VarDecl(v, init, body) =>
       var sv;
@@ -141,65 +149,79 @@ module Verifier {
         var sRhs := incarnations.REval(init.value);
         context := RSolvers.Extend(context, RExpr.Eq(RExpr.Id(sv), sRhs));
       }
-      incarnations, context, cp := ProcessStmt(body, incarnations, context, smtEngine);
+      BC.StmtMeasurePrepend(body, cont);
+      Process([body] + cont, incarnations, context, B, smtEngine);
     case Assign(lhs, rhs) =>
       var sRhs := incarnations.REval(rhs);
       var sLhs;
       incarnations, sLhs := incarnations.Update(lhs);
       context := RSolvers.Extend(context, RExpr.Eq(RExpr.Id(sLhs), sRhs));
+      Process(cont, incarnations, context, B, smtEngine);
     case Block(stmts) =>
-      var bc := context;
-      for i := 0 to |stmts|
-        invariant smtEngine.Valid()
-      {
-        incarnations, bc, cp := ProcessStmt(stmts[i], incarnations, bc, smtEngine);
-        if cp != Normal {
-          return;
-        }
-      }
+      BC.AboutStmtSeqMeasureConcat(stmts, cont);
+      Process(stmts + cont, incarnations, context, B, smtEngine);
     case Call(_, _) =>
       print "UNHANDLED STATEMENT: Call\n"; // TODO
+      Process(cont, incarnations, context, B, smtEngine);
     case Check(cond) =>
       ProveAndReport(context, incarnations.REval(cond), "check", cond, smtEngine);
+      Process(cont, incarnations, context, B, smtEngine);
     case Assume(cond) =>
       context := RSolvers.Extend(context, incarnations.REval(cond));
+      Process(cont, incarnations, context, B, smtEngine);
     case Assert(cond) =>
       var e := incarnations.REval(cond);
       ProveAndReport(context, e, "assert", cond, smtEngine);
       context := RSolvers.Extend(context, e);
+      Process(cont, incarnations, context, B, smtEngine);
     case AForall(v, body) =>
       var bodyIncarnations, _ := incarnations.Update(v);
-      bodyIncarnations, context, cp := ProcessStmt(body, bodyIncarnations, context, smtEngine);
-      expect cp.Normal?; // TODO: prove that this follows from the AForall statement satisfying its static checks
-      expect !StaticConsistency.ContainsNonAssertions(stmt); // TODO: ditto
+      BC.AboutStmtSeqMeasureSingleton(body);
+      Process([body], bodyIncarnations, context, B, smtEngine);
+
+      expect !StaticConsistency.ContainsNonAssertions(stmt); // TODO: prove that this follows from the AForall statement satisfying its static checks
       var L := Learn(stmt);
       context := RSolvers.Extend(context, incarnations.REval(L));
-    case Choice(_) =>
-      print "UNHANDLED STATEMENT: Choice\n"; // TODO
+      Process(cont, incarnations, context, B, smtEngine);
+    case Choice(branches) =>
+      for i := 0 to |branches|
+        invariant smtEngine.Valid()
+      {
+        BC.StmtSeqElement(branches, i);
+        BC.StmtMeasurePrepend(branches[i], cont);
+        Process([branches[i]] + cont, incarnations, context, B, smtEngine);
+      }
     case Loop(invariants, body) =>
-      incarnations, context, cp := ProcessLoop(stmt, incarnations, context, smtEngine);
-      if cp == Normal {
-        cp := NoExit;
-      }
+      // `cont` is ignored, since a `loop` never has any normal exit
+      ProcessLoop(stmt, incarnations, context, B, smtEngine);
     case LabeledStmt(lbl, body) =>
-      incarnations, context, cp := ProcessStmt(body, incarnations, context, smtEngine);
-      if cp == Abrupt(lbl) {
-        cp := Normal;
-      }
+      var B' := B[lbl := BC.Continuation(incarnations.Variables(), cont)];
+      BC.AboutContinuationsMeasureUpdate(B, lbl, incarnations.Variables(), cont);
+      BC.StmtPairMeasure(body, Exit(lbl));
+      Process([body, Exit(lbl)], incarnations, context, B', smtEngine);
     case Exit(lbl) =>
-      cp := Abrupt(lbl);
+      expect lbl in B; // TODO
+      var c := B[lbl];
+      var variablesInScope, cont := c.variablesInScope, c.continuation;
+      var incarnations' := incarnations.DomainRestrict(variablesInScope);
+      var B0 := B - {lbl};
+      assert B == B0[lbl := BC.Continuation(variablesInScope, cont)];
+      assert BC.ContinuationsMeasure(B) >= BC.StmtSeqMeasure(cont) + BC.ContinuationsMeasure(B0) by {
+        BC.AboutContinuationsMeasure(B0, lbl, variablesInScope, cont);
+      }
+      Process(cont, incarnations', context, B0, smtEngine);
     case Probe(e) =>
       context := RSolvers.Record(context, incarnations.REval(e));
+      Process(cont, incarnations, context, B, smtEngine);
   }
 
-  method ProcessLoop(stmt: Stmt, incarnations_in: Incarnations, context_in: RSolvers.RContext, smtEngine: RSolvers.REngine)
-      returns (incarnations: Incarnations, context: RSolvers.RContext, cp: ContinuationPoint)
+  method ProcessLoop(stmt: Stmt, incarnations_in: Incarnations, context_in: RSolvers.RContext, B: BC.T, smtEngine: RSolvers.REngine)
     requires stmt.Loop? && smtEngine.Valid()
     modifies smtEngine.Repr
     ensures smtEngine.Valid()
-    decreases stmt, 0
+    decreases BC.StmtMeasure(stmt) + BC.ContinuationsMeasure(B), 0
   {
-    incarnations, context, cp := incarnations_in, context_in, Normal;
+    var incarnations, context := incarnations_in, context_in;
 
     // Check invariants on entry
     CheckAExprs(stmt.invariants, incarnations, context, smtEngine, "invariant on entry");
@@ -220,10 +242,11 @@ module Verifier {
     // Assume invariants
     context := AssumeAExprs(stmt.invariants, incarnations, context, smtEngine);
     // Process body
-    incarnations, context, cp := ProcessStmt(stmt.body, incarnations, context, smtEngine);
-    if cp != Normal {
-      return;
-    }
+    BC.AboutStmtSeqMeasureSingleton(stmt.body);
+    Process([stmt.body], incarnations, context, B, smtEngine);
+
+    // TODO: postcondition checking should be appended to body, not checked separately
+
     // Check that invariants are maintained
     CheckAExprs(stmt.invariants, incarnations, context, smtEngine, "invariant maintained");
   }
@@ -300,200 +323,7 @@ module Verifier {
       Expr.CreateTrue()
   }
 
-/*
-  method ProcessStmt(stmt: Stmt, incarnations: Incarnations, B: BlockContinuations, o: Solver)
-    returns (incarnations': Incarnations, o': Solver)
-  {
-    match stmt
-    case VarDecl(v, init, body) =>
-      var x := incarnations.New(v);
-      Process(cont, incarnations[v := x], B, o, b3);
-    case Assign(x, rhs) =>
-      var e' := incarnations.Eval(rhs);
-      var x' := incarnations.New(x);
-      var o' := o.Extend(CreateEq(IdExpr(x'), e'));
-      Process(cont, incarnations[x := x'], B, o', b3);
-    case Block(lbl, bodyStmts) =>
-      var B' := B[lbl := Continuation(incarnations.Keys, cont)];
-      assert StmtListMeasure(stmts) + ContinuationsMeasure(B) > StmtListMeasure(bodyStmts + [Exit(lbl)]) + ContinuationsMeasure(B') by {
-        assert StmtMeasure(s0) > StmtListMeasure(bodyStmts + [Exit(lbl)]) by {
-          assert StmtMeasure(s0) == 2 + StmtListMeasure(bodyStmts);
-          AboutStmtListMeasureSingleton(Exit(lbl));
-          AboutStmtListMeasureConcat(bodyStmts, [Exit(lbl)]);
-        }
-        assert ContinuationsMeasure(B) + StmtListMeasure(cont) >= ContinuationsMeasure(B') by {
-          AboutContinuationsMeasureUpdate(B, lbl, incarnations.Keys, cont);
-        }
-
-        calc {
-          StmtListMeasure(stmts) + ContinuationsMeasure(B);
-        ==  // by assertion before `match`
-          StmtMeasure(s0) + StmtListMeasure(cont) + ContinuationsMeasure(B);
-        >  // by first assertion-by above
-          StmtListMeasure(bodyStmts + [Exit(lbl)]) + StmtListMeasure(cont) + ContinuationsMeasure(B);
-        >=  // by second assert-by above
-          StmtListMeasure(bodyStmts + [Exit(lbl)]) + ContinuationsMeasure(B');
-        }
-      }
-      WF.AboutBlockStmts(s0, b3);
-      assert WF.StmtSeq(bodyStmts + [Exit(lbl)], b3);
-      Process(bodyStmts + [Exit(lbl)], incarnations, B', o, b3);
-    case Call(name, args) =>
-      ProcessCall(name, args, cont, incarnations, B, o, b3);
-    case AForall(v, body) =>
-      WF.AboutAForall(s0, b3);
-      var x := incarnations.New(v);
-      Process([body], incarnations[v := x], B, o, b3) by {
-        assert WF.Stmt(body, b3);
-        assert StmtMeasure(s0) > StmtMeasure(body);
-        AboutStmtListMeasureSingleton(body);
-      }
-
-      var L := Learn(s0);
-      var e' := incarnations.Eval(L);
-      var o' := o.Extend(e');
-      Process(cont, incarnations, B, o', b3);
-    case If(cond, thn, els) =>
-      WF.AboutIf(s0, b3);
-      var e' := incarnations.Eval(cond);
-      var oThen := o.Extend(e');
-      Process([thn] + cont, incarnations, B, oThen, b3);
-      var oElse := o.Extend(CreateNegation(e'));
-      Process([els] + cont, incarnations, B, oElse, b3);
-    case IfCase(cases) =>
-      WF.AboutIfCase(s0, b3);
-      for i := 0 to |cases|
-        invariant CaseMeasure(s0, cases[i..]) < StmtMeasure(s0)
-      {
-        var cs := cases[i];
-        var e' := incarnations.Eval(cs.cond);
-        var o' := o.Extend(e');
-        Process([cs.body] + cont, incarnations, B, o', b3);
-      }
-    case Loop(lbl, invariants, body) =>
-      // TODO
-    case Exit(lbl) =>
-      expect lbl in B;
-      ProcessExit(lbl, incarnations, B, o, b3);
-    case Return =>
-      expect ReturnLabel in B;
-      ProcessExit(ReturnLabel, incarnations, B, o, b3);
-  }
-*/
-
 /*************************
-  method Process(stmts: seq<Stmt>, incarnations: Incarnations, B: BlockContinuations, o: Solver, b3: Program)
-    requires BValid(B, b3)
-    decreases StmtListMeasure(stmts) + ContinuationsMeasure(B)
-  {
-    if |stmts| == 0 {
-      return;
-    }
-
-    var s0, cont := stmts[0], stmts[1..];
-    assert StmtListMeasure(stmts) == StmtMeasure(s0) + StmtListMeasure(cont);
-    match s0
-    case VarDecl(v, init, body) =>
-      var x := incarnations.New(v);
-      Process(cont, incarnations[v := x], B, o, b3);
-    case Assign(x, rhs) =>
-      var e' := incarnations.Eval(rhs);
-      var x' := incarnations.New(x);
-      var o' := o.Extend(SExpr.Eq(IdExpr(x'), e'));
-      Process(cont, incarnations[x := x'], B, o', b3);
-    case Block(bodyStmts) =>
-      Process(bodyStmts + cont, incarnations, B, o, b3);
-    case Call(proc, args) =>
-      ProcessCall(proc, args, cont, incarnations, B, o, b3);
-    case Check(cond) =>
-      var e' := incarnations.Eval(cond);
-      o.Prove(e');
-      Process(cont, incarnations, B, o, b3);
-    case Assume(cond) =>
-      var e' := incarnations.Eval(cond);
-      var o' := o.Extend(e');
-      Process(cont, incarnations, B, o', b3);
-    case Assert(cond) =>
-      var e' := incarnations.Eval(cond);
-      o.Prove(e');
-      var o' := o.Extend(e');
-      Process(cont, incarnations, B, o', b3);
-    case AForall(v, body) =>
-      WF.AboutAForall(s0, b3);
-      var x := incarnations.New(v);
-      Process([body], incarnations[v := x], B, o, b3) by {
-        assert WF.Stmt(body, b3);
-        assert StmtMeasure(s0) > StmtMeasure(body);
-        AboutStmtListMeasureSingleton(body);
-      }
-
-      var L := Learn(s0);
-      var e' := incarnations.Eval(L);
-      var o' := o.Extend(e');
-      Process(cont, incarnations, B, o', b3);
-    case If(cases) =>
-      WF.AboutIfCase(s0, b3);
-      for i := 0 to |cases|
-        invariant CaseMeasure(s0, cases[i..]) < StmtMeasure(s0)
-      {
-        var cs := cases[i];
-        var e' := incarnations.Eval(cs.cond);
-        var o' := o.Extend(e');
-        Process([cs.body] + cont, incarnations, B, o', b3);
-      }
-    case Loop(lbl, invariants, body) =>
-      // TODO
-    case LabeledStmt(lbl, body) =>
-      var B' := B[lbl := Continuation(incarnations.Keys, cont)];
-      assert StmtListMeasure(stmts) + ContinuationsMeasure(B) > StmtListMeasure([body, Exit(lbl)]) + ContinuationsMeasure(B') by {
-        assert StmtMeasure(s0) > StmtListMeasure([body, Exit(lbl)]) by {
-          assert StmtMeasure(s0) == 2 + StmtMeasure(body);
-          AboutStmtListMeasureSingleton(Exit(lbl));
-          AboutStmtListMeasureConcat([body], [Exit(lbl)]); // TODO: this can probably use a more specific lemma
-        }
-        assert ContinuationsMeasure(B) + StmtListMeasure(cont) >= ContinuationsMeasure(B') by {
-          AboutContinuationsMeasureUpdate(B, lbl, incarnations.Keys, cont);
-        }
-
-        calc {
-          StmtListMeasure(stmts) + ContinuationsMeasure(B);
-        ==  // by assertion before `match`
-          StmtMeasure(s0) + StmtListMeasure(cont) + ContinuationsMeasure(B);
-        >  // by first assertion-by above
-          StmtListMeasure([body, Exit(lbl)]) + StmtListMeasure(cont) + ContinuationsMeasure(B);
-        >=  // by second assert-by above
-          StmtListMeasure([body, Exit(lbl)]) + ContinuationsMeasure(B');
-        }
-      }
-      WF.AboutBlockStmts(s0, b3);
-      assert WF.StmtSeq([body, Exit(lbl)], b3);
-      Process([body, Exit(lbl)], incarnations, B', o, b3);
-    case Exit(lbl) =>
-      expect lbl in B;
-      ProcessExit(lbl, incarnations, B, o, b3);
-    case Return =>
-      expect ReturnLabel in B;
-      ProcessExit(ReturnLabel, incarnations, B, o, b3);
-    case Probe(e) =>
-      var e' := incarnations.Eval(e);
-      var o' := o.Record(e');
-      Process(cont, incarnations, B, o', b3);
-  }
-
-  method ProcessExit(lbl: Label, incarnations: Incarnations, B: BlockContinuations, o: Solver, b3: Program)
-    requires BValid(B, b3) && lbl in B
-    decreases 1 + ContinuationsMeasure(B), 0
-  {
-      var Continuation(V, cont) := B[lbl];
-      var incarnations' := incarnations.DomainRestrict(V);
-      var B0 := B - {lbl};
-      assert B == B0[lbl := Continuation(V, cont)];
-      assert ContinuationsMeasure(B) >= StmtListMeasure(cont) + ContinuationsMeasure(B0) by {
-        AboutContinuationsMeasure(B0, lbl, V, cont);
-      }
-      Process(cont, incarnations', B0, o, b3);
-  }
-
   method ProcessCall(name: string, args: seq<CallArgument>, cont: seq<Stmt>, incarnations: Incarnations, B: BlockContinuations, o: Solver, b3: Program)
   {
     var maybeProc := b3.FindProcedure(name);
@@ -528,18 +358,6 @@ module Verifier {
     */
   }
 
-  method NewVars(vars: seq<Variable>, incarnations: Incarnations, suffix: string := "") returns (newVars: seq<Var>)
-    ensures |newVars| == |vars|
-  {
-    newVars := [];
-    for i := 0 to |vars|
-      invariant |newVars| == i
-    {
-      var y := incarnations.NewWithSuffix(vars[i], suffix);
-      newVars := newVars + [y];
-    }
-  }
-
   method CollateParameters(proc: Procedure, args: seq<CallArgument>, b3: Program) returns (
       formalIns: seq<Variable>, actualIns: seq<Expr>,
       formalInOuts: seq<Variable>, oldInOuts: seq<Variable>, actualInOuts: seq<Variable>,
@@ -559,126 +377,6 @@ module Verifier {
       match proc.parameters[i].kind
     }
     */
-  }
-
-  ghost function StmtListMeasure(stmts: seq<Stmt>): nat {
-    if stmts == [] then 0 else StmtMeasure(stmts[0]) + StmtListMeasure(stmts[1..])
-  }
-  ghost function StmtMeasure(stmt: Stmt): nat
-    ensures 0 < StmtMeasure(stmt)
-  {
-    match stmt
-    case VarDecl(_, _, _) => 1
-    case Assign(_, _) => 1
-    case Block(stmts) => StmtListMeasure(stmts)
-    case Call(_, _) => 1 // TODO
-    case Check(_) => 1
-    case Assume(_) => 1
-    case Assert(_) => 2
-    case AForall(v, body) => 1 + StmtMeasure(body)
-    case If(cases) => 1 + CaseMeasure(stmt, cases)
-    case Loop(invariants, body) => 1 + StmtMeasure(body) // TODO
-    case LabeledStmt(_, body) => 2 + StmtMeasure(body)
-    case Exit(_) => 1
-    case Probe(_) => 1
-  }
-  ghost function CaseMeasure(stmt: Stmt, cases: seq<Case>): nat
-    requires forall cs <- cases :: cs < stmt
-  {
-    if cases == [] then 0 else
-      assert cases[0] in cases && forall cs <- cases[1..] :: cs in cases;
-      StmtMeasure(cases[0].body) + CaseMeasure(stmt, cases[1..])
-  }
-
-  lemma AboutStmtListMeasureSingleton(s: Stmt)
-    ensures StmtListMeasure([s]) == StmtMeasure(s)
-  {}
-
-  lemma AboutStmtListMeasureConcat(a: seq<Stmt>, b: seq<Stmt>)
-    ensures StmtListMeasure(a + b) == StmtListMeasure(a) + StmtListMeasure(b)
-  {
-    if a == [] {
-      assert a + b == b;
-    } else {
-      assert (a + b)[0] == a[0];
-      assert (a + b)[1..] == a[1..] + b;
-    }
-  }
-
-  ghost function ContinuationsMeasure(B: BlockContinuations): nat {
-    if |B| == 0 then 0 else
-      var lbl := Pick(B.Keys);
-      StmtListMeasure(B[lbl].continuation) + ContinuationsMeasure(B - {lbl})
-  }
-  ghost function Pick<X>(s: set<X>): X
-    requires |s| != 0
-  {
-    var x :| x in s; x
-  }
-  lemma AboutContinuationsMeasure(B: BlockContinuations, x: Label, V: set<Variable>, cont: seq<Stmt>)
-    requires x !in B
-    ensures ContinuationsMeasure(B[x := Continuation(V, cont)]) == StmtListMeasure(cont) + ContinuationsMeasure(B)
-  {
-    var B' := B[x := Continuation(V, cont)];
-    assert B'[x].continuation == cont;
-    assert B' - {x} == B;
-    var y := Pick(B'.Keys);
-    if y == x {
-      assert ContinuationsMeasure(B') == StmtListMeasure(B'[x].continuation) + ContinuationsMeasure(B);
-    } else {
-      var Bxy, Bx, By, B0 := B', B' - {y}, B' - {x}, B' - {x, y};
-      assert By == B;
-      assert Bx - {x} == B0 == By - {y};
-      assert Bx == B0[x := Continuation(V, cont)];
-      assert By == B0[y := B'[y]];
-
-      var V', cont' := B'[y].V, B'[y].continuation;
-      calc {
-        ContinuationsMeasure(Bxy);
-      ==
-        StmtListMeasure(cont') + ContinuationsMeasure(Bx);
-      ==  { AboutContinuationsMeasure(B0, x, V, cont); }
-        StmtListMeasure(cont') + StmtListMeasure(cont) + ContinuationsMeasure(B0);
-      ==
-        StmtListMeasure(cont) + StmtListMeasure(cont') + ContinuationsMeasure(B0);
-      ==  { AboutContinuationsMeasure(B0, y, V', cont'); }
-        StmtListMeasure(cont) + ContinuationsMeasure(By);
-      }
-    }
-  }
-
-  lemma AboutContinuationsMeasureRemove(B: BlockContinuations, lbl: Label)
-    ensures ContinuationsMeasure(B) >= ContinuationsMeasure(B - {lbl})
-  {
-    if lbl in B {
-      var B0 := B - {lbl};
-      var V, cont := B[lbl].V, B[lbl].continuation;
-      assert B == B0[lbl := Continuation(V, cont)];
-      AboutContinuationsMeasure(B0, lbl, B[lbl].V, B[lbl].continuation);
-      assert ContinuationsMeasure(B0[lbl := Continuation(V, cont)]) == StmtListMeasure(cont) + ContinuationsMeasure(B0);
-    } else {
-      assert B == B - {lbl};
-    }
-  }
-
-  lemma AboutContinuationsMeasureUpdate(B: BlockContinuations, lbl: Label, V: set<Variable>, cont: seq<Stmt>)
-    ensures ContinuationsMeasure(B) + StmtListMeasure(cont) >= ContinuationsMeasure(B[lbl := Continuation(V, cont)])
-  {
-    var B' := B[lbl := Continuation(V, cont)];
-    if lbl in B {
-      var B0 := B - {lbl};
-      calc {
-        ContinuationsMeasure(B) + StmtListMeasure(cont);
-      >=  { AboutContinuationsMeasureRemove(B, lbl); }
-        ContinuationsMeasure(B0) + StmtListMeasure(cont);
-      >=  { AboutContinuationsMeasure(B0, lbl, V, cont); }
-        ContinuationsMeasure(B0[lbl := Continuation(V, cont)]);
-      ==  { assert B' == B0[lbl := Continuation(V, cont)] == B'; }
-        ContinuationsMeasure(B');
-      }
-    } else {
-      AboutContinuationsMeasure(B, lbl, V, cont);
-    }
   }
 *************************/
 }
