src/Verifier/BlockContinuations.dfy
@@ -1,0 +1,181 @@
+module BlockContinuations {
+  import Ast
+
+  export
+    reveals T, Continuation
+    provides Empty
+    reveals StmtMeasure
+    provides StmtSeqMeasure
+    provides AboutStmtSeqMeasureSingleton, StmtPairMeasure, StmtMeasurePrepend, StmtMeasureSplit, AboutStmtSeqMeasureConcat, StmtSeqElement
+    provides ContinuationsMeasure, AboutContinuationsMeasure, AboutContinuationsMeasureUpdate
+    provides Ast
+
+  datatype Continuation = Continuation(variablesInScope: set<Ast.Variable>, continuation: seq<Ast.Stmt>)
+
+  type T = map<Ast.Label, Continuation>
+
+  function Empty(): T {
+    map[]
+  }
+
+  ghost function StmtMeasure(stmt: Ast.Stmt): nat
+    ensures 0 < StmtMeasure(stmt)
+  {
+    match stmt
+    case VarDecl(_, _, body) => 1 + StmtMeasure(body)
+    case Assign(_, _) => 1
+    case Block(stmts) => 1 + StmtSeqMeasure(stmts)
+    case Call(_, _) => 1 // TODO
+    case Check(_) => 1
+    case Assume(_) => 1
+    case Assert(_) => 2
+    case AForall(_, body) => 1 + StmtMeasure(body)
+    case Choice(branches) => 1 + StmtSeqMeasure(branches)
+    case Loop(_, body) => 1 + StmtMeasure(body) // TODO
+    case LabeledStmt(_, body) => 2 + StmtMeasure(body)
+    case Exit(_) => 1
+    case Probe(_) => 1
+  }
+
+  ghost function StmtSeqMeasure(stmts: seq<Ast.Stmt>): nat {
+    if stmts == [] then 0 else StmtMeasure(stmts[0]) + StmtSeqMeasure(stmts[1..])
+  }
+
+  lemma StmtSeqElement(stmts: seq<Ast.Stmt>, i: nat)
+    requires i < |stmts|
+    ensures StmtMeasure(stmts[i]) <= StmtSeqMeasure(stmts)
+  {
+    if i != 0 {
+      calc {
+        StmtMeasure(stmts[i]);
+        { assert stmts[i] == stmts[1..][i - 1]; }
+        StmtMeasure(stmts[1..][i - 1]);
+      <=  { StmtSeqElement(stmts[1..], i - 1); }
+        StmtSeqMeasure(stmts[1..]);
+      <=
+        StmtSeqMeasure(stmts);
+      }
+      
+    }
+  }
+
+  lemma AboutStmtSeqMeasureSingleton(s: Ast.Stmt)
+    ensures StmtSeqMeasure([s]) == StmtMeasure(s)
+  {}
+
+  lemma StmtPairMeasure(a: Ast.Stmt, b: Ast.Stmt)
+    ensures StmtSeqMeasure([a, b]) == StmtMeasure(a) + StmtMeasure(b)
+  {
+    calc {
+      StmtSeqMeasure([a, b]);
+      { assert [a, b][1..] == [b]; }
+      StmtMeasure(a) + StmtSeqMeasure([b]);
+      { AboutStmtSeqMeasureSingleton(b); }
+      StmtMeasure(a) + StmtMeasure(b);
+    }
+  }
+
+  lemma AboutStmtSeqMeasureConcat(a: seq<Ast.Stmt>, b: seq<Ast.Stmt>)
+    ensures StmtSeqMeasure(a + b) == StmtSeqMeasure(a) + StmtSeqMeasure(b)
+  {
+    if a == [] {
+      assert a + b == b;
+    } else {
+      assert (a + b)[0] == a[0];
+      assert (a + b)[1..] == a[1..] + b;
+    }
+  }
+
+  lemma StmtMeasurePrepend(stmt: Ast.Stmt, stmts: seq<Ast.Stmt>)
+    ensures StmtSeqMeasure([stmt] + stmts) == StmtMeasure(stmt) + StmtSeqMeasure(stmts)
+  {
+    AboutStmtSeqMeasureSingleton(stmt);
+    AboutStmtSeqMeasureConcat([stmt], stmts);
+  }
+
+  lemma StmtMeasureSplit(stmts: seq<Ast.Stmt>)
+    requires stmts != []
+    ensures StmtSeqMeasure(stmts) == StmtMeasure(stmts[0]) + StmtSeqMeasure(stmts[1..])
+  {
+    assert [stmts[0]] + stmts[1..] == stmts;
+    StmtMeasurePrepend(stmts[0], stmts[1..]);
+  }
+
+  ghost function ContinuationsMeasure(B: T): nat {
+    if |B| == 0 then 0 else
+      var lbl := Pick(B.Keys);
+      StmtSeqMeasure(B[lbl].continuation) + ContinuationsMeasure(B - {lbl})
+  }
+
+  ghost function Pick<X>(s: set<X>): X
+    requires |s| != 0
+  {
+    var x :| x in s; x
+  }
+
+  lemma AboutContinuationsMeasure(B: T, x: Ast.Label, V: set<Ast.Variable>, cont: seq<Ast.Stmt>)
+    requires x !in B
+    ensures ContinuationsMeasure(B[x := Continuation(V, cont)]) == ContinuationsMeasure(B) + StmtSeqMeasure(cont)
+  {
+    var B' := B[x := Continuation(V, cont)];
+    assert B'[x].continuation == cont;
+    assert B' - {x} == B;
+    var y := Pick(B'.Keys);
+    if y == x {
+      assert ContinuationsMeasure(B') == StmtSeqMeasure(B'[x].continuation) + ContinuationsMeasure(B);
+    } else {
+      var Bxy, Bx, By, B0 := B', B' - {y}, B' - {x}, B' - {x, y};
+      assert By == B;
+      assert Bx - {x} == B0 == By - {y};
+      assert Bx == B0[x := Continuation(V, cont)];
+      assert By == B0[y := B'[y]];
+
+      var V', cont' := B'[y].variablesInScope, B'[y].continuation;
+      calc {
+        ContinuationsMeasure(Bxy);
+      ==
+        StmtSeqMeasure(cont') + ContinuationsMeasure(Bx);
+      ==  { AboutContinuationsMeasure(B0, x, V, cont); }
+        StmtSeqMeasure(cont') + StmtSeqMeasure(cont) + ContinuationsMeasure(B0);
+      ==
+        StmtSeqMeasure(cont) + StmtSeqMeasure(cont') + ContinuationsMeasure(B0);
+      ==  { AboutContinuationsMeasure(B0, y, V', cont'); }
+        StmtSeqMeasure(cont) + ContinuationsMeasure(By);
+      }
+    }
+  }
+
+  lemma AboutContinuationsMeasureRemove(B: T, lbl: Ast.Label)
+    ensures ContinuationsMeasure(B) >= ContinuationsMeasure(B - {lbl})
+  {
+    if lbl in B {
+      var B0 := B - {lbl};
+      var V, cont := B[lbl].variablesInScope, B[lbl].continuation;
+      assert B == B0[lbl := Continuation(V, cont)];
+      AboutContinuationsMeasure(B0, lbl, B[lbl].variablesInScope, B[lbl].continuation);
+      assert ContinuationsMeasure(B0[lbl := Continuation(V, cont)]) == StmtSeqMeasure(cont) + ContinuationsMeasure(B0);
+    } else {
+      assert B == B - {lbl};
+    }
+  }
+
+  lemma AboutContinuationsMeasureUpdate(B: T, lbl: Ast.Label, V: set<Ast.Variable>, cont: seq<Ast.Stmt>)
+    ensures ContinuationsMeasure(B) + StmtSeqMeasure(cont) >= ContinuationsMeasure(B[lbl := Continuation(V, cont)])
+  {
+    var B' := B[lbl := Continuation(V, cont)];
+    if lbl in B {
+      var B0 := B - {lbl};
+      calc {
+        ContinuationsMeasure(B) + StmtSeqMeasure(cont);
+      >=  { AboutContinuationsMeasureRemove(B, lbl); }
+        ContinuationsMeasure(B0) + StmtSeqMeasure(cont);
+      >=  { AboutContinuationsMeasure(B0, lbl, V, cont); }
+        ContinuationsMeasure(B0[lbl := Continuation(V, cont)]);
+      ==  { assert B' == B0[lbl := Continuation(V, cont)] == B'; }
+        ContinuationsMeasure(B');
+      }
+    } else {
+      AboutContinuationsMeasure(B, lbl, V, cont);
+    }
+  }
+}
